\documentclass[main.tex]{subfiles}

\begin{document}

\hrulefill{}

Feb 6, 2017

\vspace{3mm}
Recall
$$\mathbb{P}(A | B) = \frac{\mathbb{P}(A\cap B)}{\mathbb{P}(B)}$$
with $\mathbb{P}(A\cap B) = \mathbb{P}(A)\cdot \mathbb{P}(B)$ and $A$, $B$ independent.

Prove that if $A$ and $B$ are independent, prove $\bar{A}, B$, $A, \bar{B}$ and $\bar{A}, \bar{B}$ are all independent.

Use $\mathbb{P}(A \cap B) = \mathbb{P}(A) \cdot \mathbb{P}(B)$. Want to show that $\mathbb{P}(\bar{A} \cap B) = \mathbb{P}(\bar{A})\cdot \mathbb{P}(B)$

\begin{align}
\mathbb{P}(B) &= \mathbb{P}((A \cap B) \cup (\bar{A} \cap B)) \\
              &= \mathbb{P}(A\cap B) + \mathbb{P}(\bar{A} \cap B) \\
              &= \mathbb{P}(A)\mathbb{P}(B) + \mathbb{P}(\bar{A} \cap B) 
\end{align}
Therefore,
\begin{align}
\mathbb{P}(\bar{A} \cap B) &= \mathbb{P}(B) - \mathbb{P}(A)\mathbb{P}(B) \\
                           &= (1 - \mathbb{P}(A))\mathbb{P}(B) \\
                           &= \mathbb{P}(\bar{A})\mathbb{P}(B)
\end{align}

\subsection{Product Rule, Bayes' Rule, Law of Total Probability}

\subsubsection{Product Rule}

$$\mathbb{P}(A | B) = \frac{\mathbb{P}(A\cap B)}{\mathbb{P}(B)}$$

Therefore,
\begin{equation}
\label{eq:product-rule}
\mathbb{P}(A\cap B) = \mathbb{P}(A | B)\mathbb{P}(B)
\end{equation}

\subsubsection{Bayes' Formula}

\begin{equation}
\label{eq:bayes}
\mathbb{P}(A | B) = \frac{\mathbb{P}(A\cap B)}{\mathbb{P}(B)} = \frac{\mathbb{P}(B | A) \cdot \mathbb{P}(A)}{\mathbb{P}(B)}
\end{equation}

\begin{exmp}
10\% of population have condition $C$. There is a test that determines with some inaccuracy if you have the condition.

Test returns positive = $P$

False positive (test returns positive but they don't have the condition): 30\%
False negative (test returns negative but they do have the condition): 10\%

Want to know the probability that you have the condition if the test returns positive.

We know:

\begin{itemize}
    \item $\mathbb{P}(C) = 0.1$
    \item $\mathbb{\bar{P}} = 0.9$
    \item $\mathbb{P}(P | C) = 0.9$
    \item $\mathbb{P}(P | \bar{C}) = 0.3$
\end{itemize}

\begin{align}
\mathbb{P}(C | P) &= \frac{\mathbb{P}(P | C)\cdot\mathbb{P}(C)}{\mathbb{P}(B)}\\
                  &= \frac{\mathbb{P}(C)\mathbb{P}(P | C)}{\mathbb{P}((P \cap C) \cup (P \cap \bar{C}))}\\
                  &= \frac{\mathbb{P}(C)\mathbb{P}(P | C)}{\mathbb{P}(P\cap C) + \mathbb{P}(P \cap \bar{C})} \\
                  &= \frac{\mathbb{P}(C)\mathbb{P}(P | C)}{\mathbb{P}(C)\mathbb{P}(P | C) + \mathbb{P}(\bar{C})\mathbb{P}(P | \bar{C})} \\
                  &= \frac{0.1 * 0.9}{0.1 \cdot 0.9 + 0.1 \cdot 0.3} = 1/4
\end{align}
\end{exmp}

\end{document}
