\documentclass[main.tex]{subfiles}

\begin{document}

\section{Solving PDEs on Unbounded Domains}

\subsection{Heat equation on the line}

Feb 6, 2017

\vspace{3mm}

$u = u(x, t)$ with $u_t - ku_{xx} = 0$ and $(x, t) \in \mathbb{R} \times (0, \infty)$. Also have $u = \phi(x)$ when $(x, t) \in \mathbb{R} \times \{0\}$.

This formulation is the \mathbb{Cauchy Problem} for the heat equation. Want to find solution for $t > 0$.

Textbook:

$$\phi(x) = u_0H(x) = \begin{cases}u_0 & x \ge 0 \\ 0 & x < 0\end{cases}$$

INSERT HEAVYSIDE FIGURE


Really want to use delta ``function''

$$\phi(x) = \delta(x) = H'(x)$$

\subsubsection{Delta function}:

For any $g(x)$ continuous, $\int_{-\infty}^{\infty} g(x) \delta(x)\,dx = g(0)$
\subsubsection{Convolution}
Defining convolution: $f(x), g(x) \implies (f * g)(x) = \int_{-\infty}^{\infty} f(y) g(x - y)\,dy$

\paragraph{Letting $g = \delta$}

$$(f * \delta)(x) = \int_{-\infty}{\infty} f(y)\delta(x - y)\, dy = f(x)$$

\paragraph{Differentiating convolution}

$$(f * g)'(x) = (f * g')(x) = (f' * g)(x)$$

Suppose $G(x, t)$ solves:
$$
\begin{cases}
    G_t - kG_{xx} = 0\\
    G(x, 0) = \delta(x)
\end{cases}
$$

Suppose we have other initial data $\phi(x)$. $u(x, t) = (G * \phi)(x, t)$ with convolution in $x$ variable.

So, we can put the derivative on either variable:

\begin{align}
u_t - ku_{xx} &= G_t * \phi - kG_{xx} * \phi \\
              &= G_t - kG_{xx} * \phi = 0
\end{align}

Using this, $u(x, 0) = (\delta * \phi)(x) = \phi(x)$.

Suppose that $u$ solves with initial data $\phi(x) = u_0 H(x)$

$$u_{xt} - ku_{xxx} = {(u_x)}_t - k{(u_x)}_{xx} = {(u_t - ku_{xx})}_x = 0$$

Try to guess form of solution for this using dimensional analysis.

\begin{itemize}
    \item $u, u_0$ in degrees
    \item $x$ in length
    \item $t$ in time
    \item $k$ in $\frac{\textrm{length}^2}{\textrm{time}}$
\end{itemize}

Using the dimensionless quantities $w = \frac{u}{u_0}$, $z = \frac{x}{\sqrt{4kt}}$. Assume that $w = f(z)$

Assuming $u$, hence $w$, solves heat equation, what can we find about $f$.

\begin{align}
w_t &= f'(z)\left(\frac{-x}{2\sqrt{4kt^3}}\right) \\
w_x &= f'(z)\left(\frac{1}{\sqrt{4kt}}\right) \\
w_{xx} &= f''(z)\left(\frac{1}{4kt}\right) \\
\end{align}

Therefore,

\begin{align}
w_t - kw_{xx} &= f'(z)\frac{x}{\sqrt{4kt}}\left(\frac{-1}{2t}\right) \\
              &- kf''(z)\cdot \frac{1}{4kt}
              &= f'(z)\cdot z \cdot \left(\frac{-1}{2t}\right) \\
              &- f''(z)\cdot \frac{1}{4t} \\
              &= \frac{-1}{2t}\left(f'(z)z + \frac{1}{2}f''(z)\right) = 0
\end{align}

Then $w$ solves the PDE if $f''(z) + 2zf'(z) = 0$ (first order linear ODE in $f'$)

Multiply by $e^{z^2}\implies \left[e^{z^2}f'\right]' = 0$.

Therefore, $e^{z^2}f' = c_1 \implies f(z) = c_1\int_0^z e^{-r^2}\,dr + c_2$

Finally:
\begin{equation}
\frac{u(x,t)}{u_0} = \frac{1}{2} + \frac{1}{\sqrt{\pi}}\int_0^{x/\sqrt{4kt}} e^{-r^2}\,dr
\end{equation}

Differentiate with respect to $x$:

$$G(x, t) = \frac{1}{\sqrt{\pi}}e^{-x^2/4kt}\cdot\frac{1}{\sqrt{4kt}} = \frac{1}{\sqrt{4\pikt}} e^{-x^2/(4kt)}$$

\end{document}
