\documentclass[main.tex]{subfiles}

\begin{document}

\hrulefill{}

Feb 8, 2017

\vspace{3mm}

Recall:

$$f(0, 0) = 0, f_u (0, 0) = 0, f_\mu (0, 0) \neq 0$$

We find that $$f(u, \mu)=0$$ near (0, 0) if and only if $\mu = g(u)$.

Now, the goal is to get more information about $g(u)$

\begin{align}
\mu = g(u) &= g(0) + g'(0)u + \frac{1}{2}g''(0)u^2 + O(u^3) \\
           &= g'(0)u + \frac{1}{2}g''(0)u^2 + O(u^3)
\end{align}

$$g'(0) \neq 0 \implies \mu \approx u \implies \textrm{ linear bifurcation diagram}$$
$$g'(0) = 0 \implies \mu \approx u^2 \implies \textrm{ quadratic bifurcation diagram}$$

If $\mu = g(u)$, $\star = f(u, \mu) = f(u, g(u)) = 0$

Differentiating $\star$ with respect to $u$:

$$\star' = f_u + f_\mu\cdot g'(u) = 0$$

Evaluated at $u = 0 \implies f_u(0, 0) + f_\mu(0, 0)\cdot g'(0) = 0 = f_\mu(0, 0)g'(0)\implies g'(0) = 0$

Because of this,  $g(u) = \frac{1}{2} g''(0)u^2 + O(u^3)$.

Differentiate $\star$ one more time.

\begin{align}
\star'' &= \frac{d}{du}(f_u + f_\mu g'(u)) = 0 \\
        &= f_{uu} + f_{u\mu}g'(u) + f_{u\mu}g'(u) + f_{\mu\mu}g'^2(u) + f_u\cdot g''(u) \\
        &\implies \textrm{When u goes to 0} \\
\implies \star'' &= f_{uu} + f_\mu\cdot g''(0)
\end{align}

Therefore,

$$g''(0) = \frac{f_{uu}(0, 0)}{f_\mu (0, 0)}$$

Conclusion:

When $\frac{du}{dt} = f(u, \mu)$, assuming:
\begin{itemize}
    \item $u = 0$ is an equilibrium ($f(0, 0) = 0$)
    \item $u = 0$ is not hyperbolic ($f_u(0, 0) = 0$)
    \item $f_\mu(0, 0) \neq 0$
\end{itemize}

Then $f(u, \mu) = 0$ for $(u, \mu)$ close to $(0, 0)$ if and only if $\mu = g(u)$ for a unique $C^\infty$ function $g(u)$ and we have that $g(u) = -\frac{1}{2}\frac{f_{uu}(0,0)}{f_\mu(0, 0)}u^2 + O(u^3)$

Now we want to thnk about stability:

$f(u, \mu) = \dot{u}$ with equilibria $(u, \mu) = (u, g(u))$. Take derivative:

\begin{itemize}
    \item Stable if $f_u (u, g(u)) < 0$
    \item Unstable if $f_u (u, g(u)) < 0$
\end{itemize}

Use Taylor Expansion:

\begin{align}
    f(u, \mu) &= f + f_u\cdot u + \frac{1}{2}f_{uu}\cdot u^2 + O(\mu u + \mu^2 + u + \mu)^3 \\
              &= f_{uu}\cdot u^2 + O(|\mu| + \mu^2)
               \textrm{With } g(u) &= -\frac{1}{2}\frac{f_{uu}}{f_\mu}\cdot u^2 + O(|u|^2) \\
    f_u(u, \mu) &= f_{uu} \neq 0
\end{align}

Theorem:

Assuming:
$$\dot{u} = f(u, \mu) \textrm{ with } f(u_0, \mu_0) = 0 \textrm{ and } f_u(u_0,\mu_0) = 0, f_\mu(u_0, \mu_0) \neq 0\textrm{, and } f_{uu}(u_0, \mu_0) \neq 0$$

Then $f(u, \mu) = 0$ for $(u, \mu)$ near $(u_0, \mu_0)$ if and only if $\mu = g(u)$ for a unique $C^\infty$ function $g$ with $g(u) = \mu_0 - \frac{f_{uu}}{f_\mu} (u - u_0)^2 + O(|u - u_0|^2)$, and we have $f_u(u, g(u)) = f_{uu}(u_0, \mu_0)(u-u_0) + O(|u - u_0|^2)$ so that the sign of $f_{uu}(u_0, \mu_0)(u-u_0)$ decides on the stability of the equilibrium at $(u, \mu) = (u, g(u))$

\end{document}
